{
 "cells": [
  {
   "cell_type": "markdown",
   "metadata": {},
   "source": [
    "## 1:\n",
    "\n",
    "The density of states for a quantum particle of mass $m$ inside an infinite square well of width $a$ is\n",
    "\n",
    "$$\n",
    "\\rho_\\text{ISW} (E) = \\sum_{n=1}^{\\infty} \\delta(E - E_n), \\quad E_n = \\frac{\\hbar^2 \\pi^2}{2 ma^2}n^2, \\quad n = 1, 2...\n",
    "$$\n",
    "\n",
    "Use the energy-dependent propagator\n",
    "\n",
    "$$\n",
    "G_\\text{ISW}^{(+)}(x^\\prime, x; E) = \\frac{m}{i \\hbar^2 k} \\sum_{l = -\\infty}^{\\infty} \\left[e^{ik [x^\\prime -x + 2 al ]}- e^{ik [x^\\prime +x + 2 al ]}\\right]\n",
    "$$\n",
    "\n",
    "of the infinite square well (see eq 12.85) to verify the general trace formula\n",
    "\n",
    "$$\n",
    "\\rho(E) = - \\frac{1}{\\pi} \\Im \\text{Tr} \\hat {\\mathcal{G}}(E)\n",
    "$$"
   ]
  },
  {
   "cell_type": "markdown",
   "metadata": {},
   "source": [
    "Let's start with 14.7:\n",
    "\n",
    "$$\n",
    "\\begin{aligned}\n",
    "\\rho(E) &= - \\frac{1}{\\pi} \\Im \\int \\frac{m}{i \\hbar^2 k} \\sum_{l = -\\infty}^{\\infty} \\left[e^{ik [x^\\prime -x + 2 al ]}- e^{ik [x^\\prime +x + 2 al ]}\\right] dx \\\\\n",
    "&= -\\frac{1}{\\pi} \\Im \\left[\\frac{-im}{\\hbar^2 k} \\sum_{l=-\\infty}^{\\infty}\\int_0^a e^{2ik |al|}dx - \\int_0^a e^{2ik |x+ al|}dx\\right]\n",
    "\\end{aligned}\n",
    "$$\n",
    "\n",
    "Strictly speaking, the arguments of the above exponentials only need $l$ in absolute value bars. Let's call these integrals $I_1$ and $I_2$:\n",
    "\n",
    "$$\n",
    "I_1 = \\int_0^a e^{2ik |al|}dx = ae^{2ik|l|},\n",
    "$$\n",
    "\n",
    "and\n",
    "\n",
    "$$\n",
    "I_2 = \\int_0^a e^{2i |x + al|}dx,\n",
    "$$\n",
    "\n",
    "which has three cases:\n",
    "\n",
    "* $l=0$:\n",
    "\n",
    "$$\n",
    "I_2 = \\int_0^a e^{2i |x|}dx = \\left[\\frac{e^{2ikx}}{2ik}\\right]_0^a = \\frac{1}{2ik} (e^{2ika} -1)\n",
    "$$\n",
    "\n",
    "* $l <0$:\n",
    "\n",
    "$$\n",
    "I_2=\\int_0^a e^{2 i k(x-a l)} d x=\\frac{e^{-2 i k a l}}{2 i k}\\left(e^{2 i k a}-1\\right)\n",
    "$$\n",
    "\n",
    "* $l >0$:\n",
    "\n",
    "$$\n",
    "I_2=\\int_0^a e^{2 i k(x+a l)} d x=\\frac{e^{2 i k a l}}{2 i k}\\left(e^{2 i k a}-1\\right)\n",
    "$$"
   ]
  },
  {
   "cell_type": "markdown",
   "metadata": {},
   "source": [
    "If we put the integrals back in our $\\rho(E)$ formula we have:\n",
    "\n",
    "$$\n",
    "\\begin{aligned}\n",
    "\\rho(E) &= -\\frac{1}{\\pi} \\left(\\frac{-m}{\\hbar^2 k}\\right) \\sum_{l = -\\infty}^{\\infty}a e^{2ika |l|} \\\\\n",
    "&= \\frac{ma}{\\pi \\hbar^2 k} \\sum_{l = \\infty}^{\\infty} e^{2ika |l|}.\n",
    "\\end{aligned}\n",
    "$$\n",
    "\n",
    "Now we will use the following relations:\n",
    "\n",
    "$$\n",
    "\\delta[g(x)]=\\sum_{n=1}^N \\frac{1}{\\left|g^{\\prime}(x)\\right|} \\delta\\left(x-x_n\\right) \\\\  \\delta_ \\alpha(x)=\\sum_{n=-\\infty}^{\\infty} \\delta(x-n \\alpha) \\\\ \\delta_\\alpha(x)= \\sum_{n=-\\infty}^{\\infty} e^{2 \\pi i m x / \\alpha}\n",
    "$$\n",
    "\n",
    "Which are from eq 1.165, 1.166, and 1.191 respectively. We also donate periodicity with $\\alpha$ to avoid confusion with well width $a$. \n",
    "\n",
    "From this it's apparent that our $\\rho(E)$ looks like the periodic delta function. And thus we can recast it as:\n",
    "\n",
    "$$\n",
    "\\rho(E) = \\frac{ma}{\\pi \\hbar^2 k} \\sum_{l = -\\infty}^{\\infty} \\delta \\left(\\frac{ka}{\\pi} - |l|\\right).\n",
    "$$\n",
    "\n",
    "To apply 1.166 we need the density of states:\n",
    "\n",
    "$$\n",
    "g(E) = \\frac{\\sqrt{2mE}}{\\hbar} \\frac{a}{\\pi} - |l| \\implies g^\\prime(E) = \\frac{a}{2 \\pi} \\frac{2m}{\\hbar} \\frac{1}{\\sqrt{2mE}} = \\frac{ma}{\\pi \\hbar} \\frac{1}{\\sqrt{2m \\frac{\\hbar^2 k^2}{2m}}} = \\frac{ma}{\\pi \\hbar^2 k}\n",
    "$$"
   ]
  },
  {
   "cell_type": "markdown",
   "metadata": {},
   "source": [
    "Now notice that $\\delta(\\frac{ka}{\\pi} - |l|)$ is only non-zero at $ka = - l \\pi$, or in terms of $E = \\frac{\\hbar^2}{2m } \\left(\\frac{l \\pi}{a}\\right)^2 = \\frac{\\hbar^2 \\pi^2 l^2}{2ma^2}$, and we have chosen by calcuating $g(E)$ that $k = \\frac{\\sqrt{2mE}}{\\hbar} >0$. Since $E$ depends on $l^2$, we can throw out the negative $l$ terms in the sum. And thus\n",
    "\n",
    "$$\n",
    "\\boxed{\\rho(E) = \\frac{ma}{\\pi \\hbar^2 k} \\sum_{l=1}^{\\infty} \\frac{\\pi \\hbar^2 k }{ma} \\delta(E - E_l) = \\sum_{l = 1}^{\\infty} \\delta(E - E_l)}\n",
    "$$"
   ]
  },
  {
   "cell_type": "markdown",
   "metadata": {},
   "source": [
    "## 2:\n",
    "\n",
    "Show that\n",
    "\n",
    "$$\n",
    "\\rho(E) = \\text{Tr} \\delta(E - \\hat {\\mathcal{H}})\n",
    "$$"
   ]
  },
  {
   "cell_type": "markdown",
   "metadata": {},
   "source": [
    "To begin, write the formula for the trace:\n",
    "\n",
    "$$\n",
    "\\text{Tr} \\delta(E - \\hat{\\mathcal{H}}) = \\sum_{n=0}^{\\infty} \\langle n \\mid \\delta(E - \\hat{\\mathcal{H}}) \\mid  n \\rangle\n",
    "$$"
   ]
  },
  {
   "cell_type": "markdown",
   "metadata": {},
   "source": [
    "Because $\\hat{\\mathcal{H}} \\mid n \\rangle = E_n  \\mid n \\rangle$, and since $\\mid n \\rangle$ forms a complete and orthonormal set of states, we have that  $\\langle n\\mid  n \\rangle$ = 1. We can therefore reduce to:\n",
    "\n",
    "$$\n",
    "\\text{Tr} \\delta(E - \\hat{\\mathcal{H}}) = \\sum_{n=0}^{\\infty} \\delta(E - E_n) = \\rho(E)\n",
    "$$"
   ]
  },
  {
   "cell_type": "markdown",
   "metadata": {},
   "source": [
    "## 3:\n",
    "\n",
    "Derive the trace formula\n",
    "\n",
    "$$\n",
    "\\rho(E) = - \\frac{1}{\\pi} \\Im \\text{Tr} \\hat {\\mathcal{G}}^{(+)}(E)\n",
    "$$\n",
    "\n",
    "using the integral representation\n",
    "\n",
    "$$\n",
    "\\delta(E - \\hat {\\mathcal{H}}) = \\frac{1}{2 \\pi \\hbar} \\int_{-\\infty}^{\\infty} e^{i(E - \\hat{\\mathcal{H}})t/\\hbar} dt\n",
    "$$"
   ]
  },
  {
   "cell_type": "markdown",
   "metadata": {},
   "source": [
    "Starting with the result from question 14.2.2:\n",
    "\n",
    "$$\n",
    "\\rho(E) =\\operatorname{Tr} \\delta(E-\\hat{\\mathcal{H}})=\\operatorname{Tr} \\frac{1}{2 \\pi \\hbar} \\int_{-\\infty}^{+\\infty} e^{i(E-\\hat{\\mathcal{H}}) t / \\hbar} d t=\\operatorname{Tr} \\frac{1}{\\pi n \\hbar} \\int_0^{+\\infty} \\cos \\left[\\frac{(E-\\hat{\\mathcal{H}}) t}{\\hbar}\\right] d t \\quad \\text { (even function) } \n",
    "$$\n",
    "\n",
    "$$\n",
    "=\\operatorname{Tr} \\operatorname{Re} \\frac{1}{\\pi \\hbar} \\int_0^{\\infty} e^{i(E-\\hat{\\mathcal{H}}) t / \\hbar} d t=\\operatorname{Tr} \\operatorname{Re} \\frac{1}{\\pi \\hbar} \\int_0^{\\infty} e^{i E t / \\hbar} e^{-i \\hat{\\mathcal{H}} t / \\hbar} \\theta(t) d t \\quad\\left(\\int_0^{\\infty} f(t) d t=\\int_0^{\\infty} \\theta(t) f(t) d t\\right) \\\\\n",
    "$$\n",
    "Then use 12.28 to cast the propagator into $\\rho(E)$:\n",
    "$$\n",
    "\\hat{\\mathcal{G}}^{(+)}(t) =\\theta(t) \\exp \\left(-\\frac{i}{\\hbar} \\hat{\\mathcal{H}} t\\right).\n",
    "$$\n",
    "\n",
    "$$\\rho(E)=\\operatorname{Tr} \\operatorname{Re} \\frac{1}{\\pi \\hbar} \\int_0^{\\infty} e^{i E t / \\hbar} \\mathcal{G}^{(+)}(t) d t \\\\\n",
    "$$\n",
    "Then we can transform our time-dependent propagator to an energy-dependent propagator:\n",
    "$$\n",
    "\\hat{\\mathcal{G}}^{(+)}(E) =\\frac{1}{i \\hbar} \\int_0^{+\\infty} e^{i E t / \\hbar} \\mathcal{G}^{(+)}(t) d t\n",
    "$$\n",
    "so, \n",
    "$$\n",
    "\\rho(E)=\\operatorname{Tr} \\operatorname{Re} \\frac{i}{\\pi} \\cdot \\frac{1}{i \\hbar} \\int_0^{\\infty} e^{i E t / \\hbar} \\mathcal{G}^{(+)}(t) d t=\\operatorname{Tr} \\frac{1}{\\pi} \\operatorname{Re} i \\mathcal{G}^{(+)}(E)\n",
    "$$\n",
    "\n",
    "\n",
    "Since $\\operatorname{Re}\\{i z\\}=\\operatorname{Re}\\{i(x+i y)\\}=\\operatorname{Re}\\{i x-y\\}=-y=-\\operatorname{Im}\\{z\\}: \\rho(E)=-\\frac{1}{\\pi} \\operatorname{Im} \\operatorname{Tr} \\hat{\\mathcal{G}}^{(+)}(E)$, as desired. "
   ]
  },
  {
   "cell_type": "markdown",
   "metadata": {},
   "source": [
    "## 4:\n",
    "\n",
    "In one dimension, Weyl's formula with surface correction is\n",
    "\n",
    "$$\n",
    "N_\\text{Weyl}(E) = \\frac{a \\sqrt{2mE}}{\\pi \\hbar} - \\frac{1}{2}.\n",
    "$$\n",
    "\n",
    "(a) Compute the exact level density $\\rho(E)$ for a quantum particle of mass $m$ restricted to, but otherwise moving freely in, the interval $[0,a]$ on the $x$ axis.\n",
    "\n",
    "We showed in HW6, problem 1 (7.3.1), that the exact level density $\\rho(E)$ of a quantum particle in an infinite square well is given by:\n",
    "\n",
    "$$\n",
    "\\rho(E) = \\frac{a}{2\\pi \\hbar} \\sqrt{\\frac{2m}{ E}} \\left\\{ 1 + 2 \\sum_{m = 1}^\\infty \\cos\\left[\\frac{2 m a}{\\hbar}\\left(\\sqrt{2m E}\\right)\\right]\\right\\}\n",
    "$$"
   ]
  },
  {
   "cell_type": "markdown",
   "metadata": {},
   "source": [
    "\n",
    "(b) Compute $N(E)$ by integrating $\\rho(E)$. "
   ]
  },
  {
   "cell_type": "markdown",
   "metadata": {},
   "source": [
    "$$\n",
    "\\begin{aligned}\n",
    "N(E) &= \\int \\rho(E)dE \\\\\n",
    "& =\\int \\frac{a}{\\pi \\hbar} \\sqrt{\\frac{m}{2 E}}\\left(1+2 \\sum_{n=1}^{\\infty} \\cos \\left(\\frac{2 n a}{\\hbar} \\sqrt{2 m E}\\right)\\right) d E \\\\\n",
    "& =\\frac{a \\sqrt{m}}{\\pi \\hbar \\sqrt{2}} 2 \\sqrt{E}+\\frac{a \\sqrt{m} 2}{\\pi \\hbar \\sqrt{2 E}} \\sum_{n=1}^{\\infty}\\int \\left(\\cos \\left(\\frac{2 n a}{\\hbar} \\sqrt{2 m E}\\right) E^{-1 / 2}\\right) d E+C \\\\\n",
    "& =\\frac{a \\sqrt{2 m E}}{\\pi \\hbar}+\\sum_{n=1}^{\\infty} \\frac{1}{n \\pi} \\sin \\left[\\frac{2 a n \\sqrt{2 m E}}{\\hbar}\\right]+C,\n",
    "\\end{aligned}\n",
    "$$\n",
    "\n",
    "for integration constant $C$. \n",
    "\n",
    "We also know\n",
    "\n",
    "$$\n",
    "\\begin{aligned}\n",
    "N(E) &= \\sum_{n = 1}^{\\infty} \\Theta(E - \\frac{n^2 \\pi^2 \\hbar^2}{2 ma^2}) \\\\\n",
    "&= \\sum_{n=1}^{\\infty} \\Theta\\left(\\frac{\\pi^2 \\hbar^2}{2ma^2} - \\frac{n^2 \\pi^2 \\hbar^2}{2ma^2}\\right) \\\\\n",
    "&= \\sum_{n=1}^{\\infty} \\Theta\\left(\\frac{\\pi^2 \\hbar^2}{2ma^2} \\left(1 - n^2\\right)\\right) \\\\\n",
    "&= \\Theta(0) \\\\\n",
    "&= \\frac{1}{2}\n",
    "\\end{aligned}\n",
    "$$"
   ]
  },
  {
   "cell_type": "markdown",
   "metadata": {},
   "source": [
    "So then, we can use: \n",
    "\n",
    "$$\n",
    "N\\left(\\frac{\\pi^2 \\hbar^2}{2ma^2}\\right) = \\frac{1}{2}\n",
    "$$\n",
    "\n",
    "to determine our constant:\n",
    "\n",
    "$$\n",
    "\\frac{a\\sqrt{2m}}{\\pi \\hbar} \\frac{\\pi \\hbar}{\\sqrt{2m}a } + C +\\sum_{n=1}^{\\infty} \\frac{1}{n \\pi} \\sin \\left[\\frac{2 a n \\sqrt{2 m}}{\\hbar} \\frac{\\pi}{\\hbar\\sqrt{2m}a}\\right] = \\frac{1}{2}\n",
    "$$\n",
    "\n",
    "$$\n",
    "1 + C +\\sum_{n=1}^{\\infty} \\frac{1}{n \\pi} \\sin \\left[2n \\pi \\right] = \\frac{1}{2}\n",
    "$$\n",
    "\n",
    "$$\n",
    "1 + C  = \\frac{1}{2} \\implies C = -\\frac{1}{2}\n",
    "$$\n",
    "\n",
    "\n",
    "And thus, \n",
    "\n",
    "$$\n",
    "\\boxed{N(E) = \\frac{a \\sqrt{2 m E}}{\\pi \\hbar}+\\sum_{n=1}^{\\infty} \\frac{1}{n \\pi} \\sin \\left[\\frac{2 a n \\sqrt{2 m E}}{\\hbar}\\right]- \\frac{1}{2}}\n",
    "$$\n",
    "\n",
    "We could have also done this without integrating by simply using 7.11. "
   ]
  },
  {
   "cell_type": "markdown",
   "metadata": {},
   "source": [
    "\n",
    "(c) Discarding all oscillating terms in $N(E)$, obtain $N_\\text{Weyl}(E)$.\n",
    "All we have to do is kill the $\\sin$ term(s) and then:\n",
    "$$\n",
    "\\boxed{N(E) = \\frac{a \\sqrt{2 m E}}{\\pi \\hbar}- \\frac{1}{2}}\n",
    "$$\n"
   ]
  },
  {
   "cell_type": "markdown",
   "metadata": {},
   "source": [
    "## 5:\n",
    "\n",
    "A particle of mass $m$ moves in the potential $V(x)$. Assume that the action $S(E)$ for $V(x)$ is known, and so are the energy level $E_n$, computed according to \n",
    "\n",
    "$$\n",
    "S(E_n) = 2 \\pi \\hbar \\left(n + \\frac{1}{2} \\right), \\quad n \\geq 0 \\text{  integer}.\n",
    "$$\n",
    "\n",
    "The potential is changed to $W(x) = \\beta V(x)$, where $\\beta >0$ is a constant. Denote the energy levels of the new potential $W(x)$ by $\\tilde{E}_n$. \n",
    "\n",
    "(a) Compute an approximate, explicit formula for the energy shift $\\Delta E_n = \\tilde E_n - E_n$. \n",
    "\n",
    "We can use \n",
    "$$\n",
    "S(E) = \\oint p(x) dx = \\oint \\sqrt{2m(E-V(x))}dx\n",
    "$$, \n",
    "and similarly \n",
    "\n",
    "$$\n",
    "\\tilde S(\\tilde E) = \\oint \\sqrt{2m(\\tilde E-\\beta V(x))}dx = \\sqrt \\beta \\oint \\sqrt {2m(\\tilde E / \\beta - V(x))}dx = \\sqrt \\beta \\oint S(\\tilde E/\\beta)dx.\n",
    "$$\n",
    "\n",
    "By 14.52, we can equate these actions:\n",
    "\n",
    "$$\n",
    "\\tilde S (\\tilde E_n) = S(E_n) = 2 \\pi \\hbar\\left(n + \\frac{1}{2}\\right),\n",
    "$$\n",
    "\n",
    "and we can rewrite the action $\\tilde S (\\tilde E_n)$ like so:\n",
    "\n",
    "$$\n",
    "\\tilde S (\\tilde E_n) = \\sqrt \\beta  S(\\tilde E /\\beta) = \\sqrt\\beta S(E_n + \\tilde E_n/ \\beta - E_n),\n",
    "$$\n",
    "\n",
    "and expand:\n",
    "\n",
    "$$\n",
    "\\begin{aligned}\n",
    "\\sqrt \\beta S(\\tilde E /\\beta )& \\approx \\sqrt{\\beta}\\left(S\\left(E_n\\right)+\\left(\\frac{\\tilde{E}}{\\beta}-E_n\\right) S^{\\prime}\\left(E_n\\right)+...\\right) \\\\\n",
    "& \\approx \\sqrt{\\beta}\\left(S\\left(E_n\\right)+\\left(\\frac{\\tilde{E}}{\\beta}-E_n\\right) T\\left(E_n\\right)\\right).\n",
    "\\end{aligned}\n",
    "$$\n",
    "\n",
    "Now make the substitution: $\\tilde{E_n}=E_n+\\Delta E_n$\n",
    "\n",
    "$$\n",
    "\\begin{aligned}\n",
    "\\sqrt \\beta S(\\tilde E /\\beta )& \\approx \\sqrt{\\beta} S\\left(E_n\\right)+\\sqrt{\\beta}\\left(\\frac{E_n}{\\beta}+\\frac{\\Delta E_n}{\\beta}-E_n\\right) T\\left(E_n\\right) \\\\\n",
    "S\\left(E_n\\right) & =\\sqrt{\\beta} S\\left(E_n\\right)+\\sqrt{\\beta} T\\left(E_n\\right) E_n\\left(\\frac{1}{\\beta}-1\\right)+T\\left(E_n\\right) \\frac{\\Delta E_n}{\\sqrt{\\beta}}.\n",
    "\\end{aligned}\n",
    "$$\n",
    "\n",
    "Cool, now all we have to do is solve for $\\Delta E_n$:\n",
    "\n",
    "$$\n",
    "\\begin{aligned}\n",
    "& (1-\\sqrt{\\beta}) S\\left(E_n\\right)=\\sqrt{\\beta}   T\\left(E_n\\right) E_n\\left(\\frac{1}{\\beta}-1\\right)+T\\left(E_n\\right) \\frac{\\Delta E}{\\sqrt{\\beta}} \\\\\n",
    "& (1-\\sqrt{\\beta}) S\\left(E_n\\right)-\\sqrt{\\beta} T\\left(E_n\\right) E_n\\left(\\frac{1}{\\beta}-1\\right)=\\frac{\\Delta E}{\\sqrt{\\beta}} T\\left(E_n\\right) \\\\\n",
    "& \\sqrt{\\beta}(1-\\sqrt{\\beta}) \\frac{S\\left(E_n\\right)}{T\\left(E_n\\right)}-\\beta E_n\\left(\\frac{1}{\\beta}-1\\right)=\\Delta E_n \\\\\n",
    "& (\\sqrt{\\beta}-\\beta) \\frac{S(E_n)}{T(E_n)} - E_n\\left(\\frac{1}{\\beta}- 1 \\right)  = \\Delta E_n. \\\\\n",
    "& \\therefore \\boxed{\\Delta E_n=E_n(\\beta-1)+(\\sqrt{\\beta}-\\beta) \\frac{S\\left(E_n\\right)}{T\\left(E_n\\right)}}\n",
    "\\end{aligned}\n",
    "$$"
   ]
  },
  {
   "cell_type": "markdown",
   "metadata": {},
   "source": [
    "\n",
    "(b) For the special case of the harmonic oscillator, $V(x) = m \\omega^2 x^2/2$, your formula for $\\Delta E_n$ should be exact. Apply your formula to the harmonic oscillator and show that it is indeed exact. "
   ]
  },
  {
   "cell_type": "markdown",
   "metadata": {},
   "source": [
    "In this case, our corresponding potential $W(x) = \\beta(x)$ can be expressed as:\n",
    "\n",
    "$$\n",
    "W(x) = \\frac{\\beta}{2} m \\tilde \\omega ^2 x^2 = \\frac{1}{2} m (\\sqrt \\beta \\omega)^2x^2 = \\frac{1}{2} m \\tilde \\omega^2 x^2,\n",
    "$$\n",
    "\n",
    "where $\\tilde \\omega = \\sqrt \\beta \\omega$. \n",
    "\n",
    "And we know the energy levels of a harmonic oscillator (4.55):\n",
    "\n",
    "$$\n",
    "E_n = \\hbar \\omega \\left(n + \\frac{1}{2}\\right),\n",
    "$$\n",
    "\n",
    "$$\n",
    "\\tilde E_n = \\hbar \\tilde \\omega \\left(n + \\frac{1}{2}\\right) = \\sqrt \\beta \\hbar \\omega \\left(n + \\frac{1}{2}\\right) = \\sqrt \\beta E_n,\n",
    "$$\n",
    "\n",
    "and thus\n",
    "\n",
    "$$\n",
    "\\Delta E_n  = \\sqrt \\beta E_n - E_n = E_n (\\sqrt \\beta -1).\n",
    "$$\n",
    "\n",
    "Let's verify this with the formula we found in part (a):\n",
    "\n",
    "$$\n",
    "E_n=E_n(\\beta-1)+(\\sqrt{\\beta}-\\beta) \\frac{S\\left(E_n\\right)}{T\\left(E_n\\right)}.\n",
    "$$\n",
    "\n",
    "We can plug in the action for one cycle of the harmonic oscillator (5.19):\n",
    "\n",
    "$$\n",
    "S(E) = 2 \\pi E / \\omega \\implies T(E) = \\frac{2\\pi}{\\omega} \\implies \\frac{S(E)}{T(E)} = E_n,\n",
    "$$\n",
    "\n",
    "so then:\n",
    "\n",
    "$$\n",
    "\\begin{aligned}\n",
    "\\Delta E_n &= \\beta E_n - E_n + E_n (\\sqrt{\\beta}) -\\beta E_n. \\\\\n",
    " &= \\sqrt{\\beta}E_n  - E_n \\\\\n",
    " &= E_n(\\sqrt{\\beta} -1), \\\\\n",
    "\\end{aligned}\n",
    "$$\n",
    "which is just we expected to find. "
   ]
  },
  {
   "cell_type": "markdown",
   "metadata": {},
   "source": [
    "## 6:\n",
    "\n",
    "Energy-scaling systems are an important class of systems for which the action $S_l(E)$ of a periodic orbit can be written as $S_l(E) = \\sigma_l f(E)$, where $\\sigma_l$ is a constant and $f(E)$ is known, for instance from considering the Weyl formulas. For these systems, Gutzwiller's trace formula can be written in the form\n",
    "\n",
    "$$\n",
    "\\rho(E) = \\sum_n \\delta(E- E_n) \\approx \\sum_l A_lT_l(E)E^{i S_l (E)/\\hbar},\n",
    "$$\n",
    "\n",
    "where the $l$-sum is over the periodic orbits of the system, $A_l$ is a constant, and \n",
    "\n",
    "$$\n",
    "T_l(E) = \\frac{\\partial S_l (E)}{\\partial E}.\n",
    "$$\n",
    "\n",
    "It is sometimes very difficult to find the actions of the classical periodic orbits. Suprisingly, in such cases, and for energy-scaling systems, quantum mechanics may behelpful to determine the actions of the classical periodic orbits. Assume that $\\rho(E)$ is known, either determined experimentally by spectroscopy or numerically by solving the Schr√∂dinger equation. In addition, assume that $f(E)$, too, is known. Then, show that\n",
    "\n",
    "$$\n",
    "F (\\sigma) = \\int_0^{E_\\text{max}} \\rho(E) e^{-i \\sigma f(E)/\\hbar}dE\n",
    "$$\n",
    "\n",
    "is sharply peaked on the action constants $\\sigma_l$ of the classical periodic orbits, where $f(E_\\text{max})$ is large and $f(0) = 0$. Let $N(E)$ be the staircase function. Would considering\n",
    "\n",
    "$$\n",
    "G(\\sigma) = \\int_0^{E_\\text{max}} N(E) e^{-i \\sigma f(E)/\\hbar}dE\n",
    "$$\n",
    "\n",
    "be a better choice?"
   ]
  },
  {
   "cell_type": "markdown",
   "metadata": {},
   "source": [
    "To begin, calculate $F(\\sigma)$:\n",
    "$$\n",
    "\\begin{aligned}\n",
    "& F(\\sigma)=\\int_0^{E_{\\text {non }}} \\rho(E) e^{-i \\sigma f(E)} d E \\\\\n",
    "& =\\int_0^{E_{\\text {max }}} \\sum_l A_l \\frac{\\partial S_l(E)}{\\partial E} e^{\\frac{i}{\\hbar} \\left[S_l(E)-\\sigma f(E)\\right]} d E \\\\\n",
    "& =\\int_0^{E_{\\text {max }}} \\sum_l A_l \\sigma_l f^{\\prime}(E) e^{\\frac{i}{\\hbar} \\left[\\sigma_l-\\sigma\\right] f(E) } dE\\\\\n",
    "& =\\sum_l A_l \\sigma_l \\frac{1}{\\left(\\frac{i}{\\hbar}\\right)\\left[\\sigma_l-\\sigma\\right]}\\left\\{e^{\\frac{i}{i}\\left[\\sigma_l-\\sigma\\right] f\\left(E_{\\text {max }}\\right)}-1\\right\\} \\\\\n",
    "& =\\sum_l A_l \\sigma_l \\frac{e^{\\frac{i}{2 \\hbar}\\left[\\sigma_l-\\sigma\\right] f\\left(E_{\\text {max }}\\right)}}{\\frac{i}{2 \\hbar}\\left[\\sigma_l-\\sigma\\right] \\cdot 2}\\left\\{e ^{\\frac{i}{2\\hbar} [\\sigma_l - \\sigma]f(E_\\text{max})} - e^{- \\frac{i}{2\\hbar} [\\sigma_l - \\sigma] f(E_\\text{max})}\\right\\} \\\\\n",
    "& =\\pi \\sum_l A_l \\sigma_l e^{\\frac{i}{2 \\hbar}\\left[\\sigma_l-\\sigma\\right] f\\left(E_{\\text {max }}\\right)} \\frac{\\sin \\left[\\frac{\\left(\\sigma_l-\\sigma\\right)}{2 \\hbar} \\cdot f\\left(E_{\\text {max }}\\right)\\right]}{\\pi\\left(\\frac{\\sigma_l-\\sigma}{2 \\hbar}\\right)}\n",
    "\\end{aligned}\n",
    "$$"
   ]
  },
  {
   "cell_type": "markdown",
   "metadata": {},
   "source": [
    "Recall that one such representation of the $\\delta$-function is\n",
    "\n",
    "$$\n",
    "\\lim_{c \\to \\infty}\\frac{1}{\\pi} \\frac{\\sin (c x)}{x}\n",
    "$$\n",
    "\n",
    "by eq 1.163. \n",
    "\n",
    "So we can then rewrite $F(\\sigma)$:\n",
    "\n",
    "$$\n",
    "\\begin{aligned}\n",
    "F(\\sigma )& =\\pi \\sum_l A_l \\sigma_l e^{\\frac{i}{2 \\hbar}\\left[\\sigma_l-\\sigma\\right] f\\left(E_{\\text {max }}\\right)} {\\delta\\left(\\frac{\\sigma_l-\\sigma}{2 \\hbar}\\right)} \\\\\n",
    "&= 2 \\pi \\hbar \\sum_l A_l \\sigma_l e^{i/2\\hbar [\\sigma_l - \\sigma] f(E_\\text{max})} \\delta(\\sigma_l - \\sigma) \\\\\n",
    "&= 2 \\pi \\hbar \\sum_l A_l \\sigma_l  \\delta(\\sigma_l - \\sigma).\n",
    "\\end{aligned}\n",
    "$$\n",
    "\n",
    "This last step is justified because the $\\delta$-function will only contribute when $\\sigma_l = \\sigma$, and otherwise that factor will be 1. Hence, \n",
    "\n",
    "$$\n",
    "F(\\sigma) = 2 \\pi \\hbar \\sum_l A_l \\sigma_l \\delta(\\sigma_l - \\sigma),\n",
    "$$\n",
    "\n",
    "which is sharply peaked at $\\sigma = \\sigma_l$. "
   ]
  },
  {
   "cell_type": "markdown",
   "metadata": {},
   "source": [
    "---\n",
    "\n",
    "Now, what happens when we use $N(E)$ instead of $\\rho(E)$?\n",
    "\n",
    "Similar to above, we show:\n",
    "\n",
    "$$\n",
    "\\begin{aligned}\n",
    "& N(E)=\\int_0^E \\rho\\left(E^{\\prime}\\right) d E^{\\prime}=\\int_0^E \\sum_l A_l T_l\\left(E^{\\prime}\\right) e^{\\frac{i}{\\hbar} S_l\\left(E^{\\prime}\\right)} d E^{\\prime} \\\\\n",
    "= & \\sum_l A_l \\int_0^E \\sigma_l f^{\\prime}\\left(E^{\\prime}\\right) e^{\\frac{i}{\\hbar} \\sigma_l f\\left(E^{\\prime}\\right)} d E^{\\prime} \\\\\n",
    "= & \\sum_l A_l \\sigma_l \\frac{1}{\\left(\\frac{i}{\\hbar}\\right) \\sigma_l}\\left\\{e^{\\frac{i}{\\hbar} \\sigma_l f(E)}-1\\right\\} .\n",
    "\\end{aligned}\n",
    "$$"
   ]
  },
  {
   "cell_type": "markdown",
   "metadata": {},
   "source": [
    "Armed with this, we compute:\n",
    "\n",
    "$$\n",
    "\\begin{aligned}\n",
    "G (\\sigma) &= \\int_0^{E_\\text{max}}N(E^\\prime) e^{- \\frac{i}{\\hbar} \\sigma f(E ^\\prime)}d E^\\prime \\\\\n",
    "&= \\int_0^{E_\\text{max}} \\sum_l A_l \\frac{1}{\\frac{i}{\\hbar} \\sigma_l} \\left\\{ e^{\\frac{i}{\\hbar} \\sigma_l f(E^\\prime)} - 1 \\right\\}e^{-\\frac{i}{\\hbar} \\sigma f(E^\\prime)}dE^\\prime\n",
    "\\end{aligned}\n",
    "$$"
   ]
  },
  {
   "cell_type": "markdown",
   "metadata": {},
   "source": [
    "And here we are stuck. Granted, the problem tells us what $f(E^\\prime)$ is, but since the factor of $f^\\prime(E)$ is no longer in the integral, we cannot go further unless we know the explict formula for $f(E^\\prime)$. So no, this method is not a better choice. "
   ]
  }
 ],
 "metadata": {
  "authors": [
   {
    "name": "Max Hanrahan"
   }
  ],
  "kernelspec": {
   "display_name": "Python 3 (ipykernel)",
   "language": "python",
   "name": "python3"
  },
  "language_info": {
   "codemirror_mode": {
    "name": "ipython",
    "version": 3
   },
   "file_extension": ".py",
   "mimetype": "text/x-python",
   "name": "python",
   "nbconvert_exporter": "python",
   "pygments_lexer": "ipython3",
   "version": "3.12.2"
  }
 },
 "nbformat": 4,
 "nbformat_minor": 4
}
